pushing towards swapping Genvs

src/GenvSwap.v
@@ -21,18 +21,31 @@ Require Import EricTact.
 
 Require Import Cmajor.
 
+Definition mem_of_state (st : Cminor.state) : mem :=
+  match st with
+  | Cminor.State _ _ _ _ _ m => m
+  | Cminor.Callstate _ _ _ m => m
+  | Cminor.Returnstate _ _ m => m
+  end.
+
 Section GENVSWAP.
 
   Variable st st' : Cminor.state.
   Variable prog : Cminor.program.
   Variable fv av rv : value.
+  Variable t : trace.
+  Definition ge := Genv.globalenv prog.
+
+  (* execution of the original Oeuf program *)
   Hypothesis start : cminor_is_callstate prog fv av st.
   Hypothesis finish : cminor_final_state prog st' rv.
-  Definition ge := Genv.globalenv prog.
-  Variable t : trace.
   Hypothesis exec : star Cminor.step ge st t st'.
 
+  (* new wider global environment *)
   Variable tge : Genv.t Cminor.fundef unit.
+
+  (* widening obligations *)
+  Hypothesis nfp : no_future_pointers (mem_of_state st).
 
   Hypothesis symb : forall id b,
       Genv.find_symbol ge id = Some b ->
@@ -71,6 +84,44 @@ Section GENVSWAP.
     destruct arg'; destruct op; simpl in *; try congruence; eexists; split; try reflexivity; inv H; eauto.
   Qed.
 
+  Lemma lessdef_cmpu :
+    forall m m',
+      Mem.inject (Mem.flat_inj (Mem.nextblock m)) m m' ->
+      forall a b c,
+        Val.lessdef (Val.cmpu (Mem.valid_pointer m) c a b) (Val.cmpu (Mem.valid_pointer m') c a b).
+  Proof.
+    intros.
+    assert (Hvp : forall b ofs, Mem.valid_pointer m b ofs = true -> Mem.valid_pointer m' b ofs = true). {
+      intros.
+      eapply Mem.valid_pointer_inject in H0; try eassumption.
+      erewrite Z.add_0_r in H0. eassumption.
+      unfold Mem.flat_inj.
+      unfold Mem.valid_pointer in *.
+      unfold Mem.perm_dec in *.
+      unfold Mem.perm_order'_dec in *.
+      unfold proj_sumbool in *.
+      break_match_hyp; try congruence.
+      unfold Mem.perm_order' in *.
+      break_match_hyp; try solve [inv p].
+      break_match; try reflexivity.
+      eapply Mem.nextblock_noaccess in n.
+      erewrite n in Heqo. congruence.
+    }
+    
+    destruct c eqn:?; unfold Val.cmpu; unfold Val.cmpu_bool; simpl;
+    repeat (break_match; try congruence; simpl);
+    try solve [try econstructor; eauto];
+    repeat 
+      (try rewrite andb_true_iff in *;
+       try rewrite andb_false_iff in *;
+       try rewrite orb_false_iff in *;
+       try rewrite orb_true_iff in *);
+       repeat progress (try break_or; try break_and);
+         try congruence;
+       match goal with
+       | [ H : Mem.valid_pointer m ?X ?Y = true, H2 : Mem.valid_pointer m' ?X ?Y = false |- _ ] => eapply Hvp in H; congruence
+       end.
+  Qed.
 
   Lemma lessdef_binop :
     forall op a a' b b' res m m',
@@ -93,28 +144,9 @@ Section GENVSWAP.
             end;
             eauto].
 
-    admit.
-    (*
-    destruct c; simpl in *;
-      unfold Val.cmpu;
-      unfold Val.cmpu_bool;
-      repeat break_match;
-      try congruence;
-      try solve [eauto].
-    rewrite andb_true_iff in *.
-    break_and. rewrite H3 in *.
-    simpl in Heqb0.
-    rewrite orb_true_iff in H4.
-    rewrite <- Mem.weak_valid_pointer_spec in H4.
-    eapply Mem.weak_valid_pointer_inject in H4; try eapply H2.
-    instantiate (1 := 0) in H4. rewrite Z.add_0_r in *.
-    rewrite orb_false_iff in Heqb0. break_and.
-    rewrite Mem.weak_valid_pointer_spec in H4.
-    destruct H4.
-    rewrite H4 in e. congruence.
-    rewrite H4 in e0. congruence.*)
-    
-  Admitted.
+    simpl. eexists; split; try reflexivity.
+    eapply lessdef_cmpu; eauto.
+  Qed.
 
   Definition match_env (e e' : Cminor.env) : Prop :=
     forall id v,
@@ -122,7 +154,6 @@ Section GENVSWAP.
       exists v',
         PTree.get id e' = Some v' /\ Val.lessdef v v'.
 
-  
   Lemma eval_expr_transf :
     forall sp e m a v m' e',
       Cminor.eval_expr ge sp e m a v ->
@@ -204,40 +235,143 @@ Section GENVSWAP.
     subst. eapply ffp; eauto.
   Qed.
 
+  Inductive match_cont : Cminor.cont -> Cminor.cont -> Prop :=
+  | match_stop :
+      match_cont Cminor.Kstop Cminor.Kstop
+  | match_seq :
+      forall k k' s,
+        match_cont k k' ->
+        match_cont (Cminor.Kseq s k) (Cminor.Kseq s k')
+  | match_block :
+      forall k k',
+        match_cont k k' ->
+        match_cont (Cminor.Kblock k) (Cminor.Kblock k')
+  | match_call :
+      forall k k' e e' oid f sp,
+        match_cont k k' ->
+        match_env e e' ->
+        match_cont (Cminor.Kcall oid f sp e k) (Cminor.Kcall oid f sp e' k').
   
   Inductive match_states : Cminor.state -> Cminor.state -> Prop :=
   | match_state :
-      forall f s k v e e' m m',
+      forall f s k k' v e e' m m',
         match_env e e' ->
+        match_cont k k' ->
         Mem.inject (Mem.flat_inj (Mem.nextblock m)) m m' ->
+        Mem.nextblock m = Mem.nextblock m' ->
         (Cminor.fn_stackspace f) > 0 ->
         match_states (Cminor.State f s k v e m)
-                     (Cminor.State f s k v e' m')
+                     (Cminor.State f s k' v e' m')
   | match_callstate :
-      forall fd vs k m vs' m',
+      forall fd vs k k' m vs' m',
         Mem.inject (Mem.flat_inj (Mem.nextblock m)) m m' ->
+        Mem.nextblock m = Mem.nextblock m' ->
         Val.lessdef_list vs vs' ->
+        match_cont k k' ->
         match_states (Cminor.Callstate fd vs k m)
-                     (Cminor.Callstate fd vs' k m')
+                     (Cminor.Callstate fd vs' k' m')
   | match_returstate :
-      forall v v' k m m',
+      forall v v' k k' m m',
         Val.lessdef v v' ->
+        match_cont k k' ->
+        Mem.nextblock m = Mem.nextblock m' ->
         Mem.inject (Mem.flat_inj (Mem.nextblock m)) m m' ->
         match_states (Cminor.Returnstate v k m)
-                     (Cminor.Returnstate v' k m').
+                     (Cminor.Returnstate v' k' m').
+
+  Lemma match_call_cont :
+    forall k k',
+      match_cont k k' ->
+      Cminor.is_call_cont k ->
+      Cminor.is_call_cont k'.
+  Proof.
+    induction k; intros; inv H; eauto.
+  Qed.
+  
+  Lemma mem_free :
+    forall m m',
+      Mem.inject (Mem.flat_inj (Mem.nextblock m)) m m' ->
+      Mem.nextblock m = Mem.nextblock m' ->
+      forall b hi m0,
+        hi > 0 ->
+        Mem.free m b 0 hi = Some m0 ->
+        exists m0',
+          Mem.free m' b 0 hi = Some m0' /\ Mem.inject (Mem.flat_inj (Mem.nextblock m0)) m0 m0' /\ Mem.nextblock m0 = Mem.nextblock m0'.
+  Proof.
+    intros.
+    assert (Hfree : Mem.nextblock m = Mem.nextblock m0) by (eapply Mem.nextblock_free in H2; congruence).
+    eapply Mem.free_parallel_inject in H2; eauto.
+    Focus 2.
+        unfold Mem.flat_inj.
+        app Mem.free_range_perm Mem.free.
+        unfold Mem.range_perm in *.
+        assert (Mem.perm m b 0 Cur Freeable) by (eapply H2; omega).
+        eapply Mem.perm_valid_block in H4.
+        unfold Mem.valid_block in *.
+        break_match; try congruence.
+        reflexivity.
+        break_exists. break_and. repeat rewrite Z.add_0_r in *.
+        eexists; split. eauto.
+        split. 
+
+      eapply Mem.nextblock_free in H2.
+      congruence.
+      eapply Mem.nextblock_free in H2.
+      congruence.
+  Qed.
+
+  Lemma mem_storev :
+    forall m m',
+      Mem.inject (Mem.flat_inj (Mem.nextblock m)) m m' ->
+      Mem.nextblock m = Mem.nextblock m' ->
+      forall c vaddr vaddr' v v' m0,
+        Val.lessdef v v' ->
+        Val.lessdef vaddr vaddr' ->
+        Mem.storev c m vaddr v = Some m0 ->
+        exists m0',
+          Mem.storev c m' vaddr' v' = Some m0' /\ Mem.inject (Mem.flat_inj (Mem.nextblock m0)) m0 m0' /\ Mem.nextblock m0 = Mem.nextblock m0'.
+  Proof.
+    
+  Admitted.
+
+  (*
+  Definition wf_local_env (e : env) (b : block) : Prop :=
+    forall id ofs b',
+      e ! id = Some (Vptr b' ofs) ->
+      Plt b' b.
+
+  
+  Definition wf_global_env (ge : Genv.t Cminor.fundef unit) (b : block) : Prop :=
+    forall id b',
+      Genv.find_symbol ge id = Some b' ->
+      Plt b' b.
+
 
   Lemma eval_expr_ptr :
     forall sp e m' m a b ofs,
       Cminor.eval_expr tge sp e m' a (Vptr b ofs) ->
+      wf_local_env e (Mem.nextblock m) ->
+      wf_global_env tge (Mem.nextblock m) ->
       Mem.inject (Mem.flat_inj (Mem.nextblock m)) m m' ->
       Plt b (Mem.nextblock m).
   Proof.
-    induction 1; intros.
-    admit. (* have to thread through env *)
-     (* HERE *)
-    intros.
   Admitted.
-
+   *)
+  Lemma match_env_set :
+    forall e e',
+      match_env e e' ->
+      forall id v x,
+        Val.lessdef v x ->
+        match_env (PTree.set id v e) (PTree.set id x e').
+  Proof.
+    intros.
+    unfold match_env.
+    intros.
+    destruct (peq id id0); try subst;
+      repeat rewrite PTree.gss in *;
+      repeat rewrite PTree.gso in * by congruence;
+      try find_inversion; eauto.
+  Qed.
   
   Lemma step_sim :
     forall st t st' st0,
@@ -248,70 +382,32 @@ Section GENVSWAP.
   Proof.
     intros.
     inv H; inv H0;
-      try eapply eval_expr_transf in H0; eauto;
-        try eapply eval_expr_transf in H1; eauto;
-          try eapply eval_expr_transf in H2; eauto;
-            try eapply eval_expr_transf in H3; eauto;
-          repeat break_exists; repeat break_and;
-            try solve [eexists; split; simpl; try econstructor; eauto].
-    (*
-    - eapply Mem.free_parallel_inject in H2; eauto.
-      Focus 2.
-      unfold Mem.flat_inj. 
-      app Mem.free_range_perm Mem.free.
-      unfold Mem.range_perm in H2.
-      assert (Mem.perm m sp 0 Cur Freeable) by (eapply H2; omega).
-      eapply Mem.perm_valid_block in H4.
-      unfold Mem.valid_block in *.
-      break_match; try congruence.
-      reflexivity.
-      break_exists. break_and. repeat rewrite Z.add_0_r in *.
-      eexists; split; econstructor. eauto. eauto.
-      eauto.
-      admit. (* nextblock m = nextblock m' is necessary *)
+      match goal with
+      | [ H : match_cont _ _ |- _ ] => inversion H; [idtac]
+      | [ |- _ ] => idtac
+      end;
+      try subst;
+    repeat match goal with
+           | [ H : Cminor.eval_expr ge _ _ _ _ _ |- _ ] => eapply eval_expr_transf in H; eauto
+           | [ H : Cminor.eval_exprlist ge _ _ _ _ _ |- _ ] => eapply eval_exprlist_transf in H; eauto
+           end;
+    repeat break_exists; repeat break_and;
+      try app mem_free Mem.free;
+      try app mem_storev Mem.storev;
+      try solve [eexists; split; simpl; try econstructor; eauto; try eapply match_call_cont; eauto; try eapply match_env_set; eauto; try econstructor; eauto].
 
-      
-    - unfold Mem.storev in *. break_match_hyp; try congruence.
+    
+    - eexists; split; simpl; try econstructor; eauto.
+      unfold Genv.find_funct in *.
+      repeat break_match_hyp; try congruence.
       inv H5.
-      assert (Hinj : Mem.flat_inj (Mem.nextblock m) b = Some (b, 0)).
-      {
-        unfold Mem.flat_inj.
-        app Mem.store_valid_access_3 Mem.store.
-        eapply Mem.valid_access_implies in H3;
-          try eapply Mem.valid_access_valid_block in H3;
-          try solve [econstructor].
-        unfold Mem.valid_block in *.
-        break_match; congruence.
-      }
-      app Mem.store_mapped_inject Mem.store;
-        try instantiate (1 := x).
-      rewrite (Z.add_0_r) in *.
-      eexists; econstructor; eauto.
-      inv H4; try econstructor; eauto.
-      destruct x; try econstructor; eauto.
-      
-      instantiate (1 := 0). admit. admit.
-      (* bring this in from somewhere *)
-      
-      SearchAbout Mem.inject.
-      eexists; econstructor; eauto.
-      
-      
-    
-    
-    
-    eexists; econstructor. eauto.
-    SearchAbout Mem.free.
-        try solve [eexists; split; try solve [econstructor; eauto]; eauto].
-      try app eval_expr_transf Cminor.eval_expr.
-      try eapply eval_expr_transf; eauto;
-        try eapply eval_exprlist_transf; eauto;
-          try eapply find_funct_transf; eauto.
-            eapply external_call_symbols_preserved_gen; try eassumption.
-    
+      break_match; try congruence.
+      eapply ffp; eauto.
+      econstructor; eauto.
 
-    SearchAbout external_call.
-     *)
+    - 
+
+      
   Admitted.
 
       
